chapter06/solutions/protocol.i.dfy
@@ -8,33 +8,33 @@ datatype Message = Grant(dest:HostId, epoch:nat)
 // Define your Host protocol state machine here.
 datatype HostState = HostState(holdsLock:bool, epoch:nat)
 
-predicate HostInit(s:HostState, id:HostId) {
-  && s.holdsLock == (id == 0)
-  && s.epoch == if id == 0 then 1 else 0
+predicate HostInit(v:HostState, id:HostId) {
+  && v.holdsLock == (id == 0)
+  && v.epoch == if id == 0 then 1 else 0
 }
 
-predicate DoGrant(s:HostState, s':HostState, a:NetAction<Message>, recipient:HostId) {
-  && s.holdsLock == true
+predicate DoGrant(v:HostState, v':HostState, a:NetAction<Message>, recipient:HostId) {
+  && v.holdsLock == true
   && a.rcv.None?
-  && a.send == {Grant(recipient, s.epoch + 1)}
-  && s'.holdsLock == false
-  && s'.epoch == s.epoch
+  && a.send == {Grant(recipient, v.epoch + 1)}
+  && v'.holdsLock == false
+  && v'.epoch == v.epoch
 }
 
-predicate DoAccept(id:HostId, s:HostState, s':HostState, a:NetAction<Message>) {
+predicate DoAccept(id:HostId, v:HostState, v':HostState, a:NetAction<Message>) {
   && a.rcv.Some?
   && a.rcv.value.dest == id
-  && a.rcv.value.epoch > s.epoch
+  && a.rcv.value.epoch > v.epoch
   && a.send == {}
-  && s'.epoch == a.rcv.value.epoch
-  && s'.holdsLock == true
+  && v'.epoch == a.rcv.value.epoch
+  && v'.holdsLock == true
 }
 
 // The (trusted) DistributedSystem helpfully tells the host what its id is,
 // so the host can tell which messages are addressed to it. In a real system,
 // that id would be a constant part of the hosts' state; here we're trying
 // to keep the boilerplate to a minimum.
-predicate HostNext(id:HostId, s:HostState, s':HostState, a:NetAction<Message>) {
-  || (exists recipient :: DoGrant(s, s', a, recipient) )
-  || DoAccept(id, s, s', a)
+predicate HostNext(id:HostId, v:HostState, v':HostState, a:NetAction<Message>) {
+  || (exists recipient :: DoGrant(v, v', a, recipient) )
+  || DoAccept(id, v, v', a)
 }
