chapter06/exercises/exercise01.dfy
@@ -8,8 +8,8 @@
 //increasing epoch number with the lock. Initially, node 0 holds the lock and
 //its epoch number is 1. A node that holds the lock can “grant” it to another
 //node by sending them a “Grant” message which has an epoch number that is
-//greater than the node’s epoch number. A node that receives such a message
-//will become the new holder and will set its epoch number to the message’s
+//greater than the node’v epoch number. A node that receives such a message
+//will become the new holder and will set its epoch number to the message’v
 //epoch number.
 
 // You'll first need to modify 'protocol.i.dfy' to define the protocol message
@@ -21,18 +21,18 @@ include "distributed_system.s.dfy"
 
 // Replace 'false' with an appropriate safety condition: no two clients hold
 // the lock simulatneously.
-predicate Safety(s:DistState) {
+predicate Safety(v:DistState) {
   false
 }
 
 // Replace 'true' with an invariant that's induction and supports Safety.
-predicate Inv(s:DistState) {
+predicate Inv(v:DistState) {
   true
 }
 
 lemma SafetyProof()
-  ensures forall s :: DistInit(s) ==> Inv(s)
-  ensures forall s, s' :: Inv(s) && DistNext(s, s') ==> Inv(s')
-  ensures forall s :: Inv(s) ==> Safety(s)
+  ensures forall v :: DistInit(v) ==> Inv(v)
+  ensures forall v, v' :: Inv(v) && DistNext(v, v') ==> Inv(v')
+  ensures forall v :: Inv(v) ==> Safety(v)
 {
 }
